checker-isa19/ShortestPathNegCVerification.thy
@@ -2014,31 +2014,6 @@ proof -
         (simp add: abs_IDist_def)+)
 qed
 
-lemma range:
-  fixes x :: word32
-  assumes a1: "sint x < 0"
-  assumes a2: "uint x \<le> INT_MAX"
-  shows "False"
-proof-
-  have "sint x \<le> (2::int)^31 - 1"
-    using a1 by auto
-  then have "uint x \<le> (2::int)^31 - 1"
-    using a2 INT_MAX_def by simp
-  then have "0 \<le> sint x" sorry
-  show ?thesis sorry
-qed
-
-lemma range_2:
-  fixes x :: word32
-  assumes a1: "\<not> int (unat x) \<le> INT_MAX"
-  shows "sint x < 0"
-proof-
-  have "int (unat x ) > INT_MAX"
-    using a1 by linarith
-  show ?thesis sorry
-qed
-  
-
 definition s_assms_inv :: "IGraph \<Rightarrow> IVertex \<Rightarrow> IENInt \<Rightarrow> IPEdge \<Rightarrow> IEInt \<Rightarrow> bool" where
   "s_assms_inv G sc d p n \<equiv> 
       (sc < ivertex_cnt G) \<and>
@@ -2086,17 +2061,18 @@ lemma s_assms_spc':
        apply (unfold is_pedge_def is_graph_def s_assms_inv_def)[1]
        apply clarsimp
        apply (subgoal_tac "iP sc = heap_w32 s (PTR_COERCE(32 signed word \<rightarrow> 32 word) (p +\<^sub>p uint sc))")
-        apply clarsimp 
-        apply(blast intro: range)
+        apply clarsimp
+        apply (metis sint_ucast)
        apply (blast intro: pedge_abs_C_equiv_2)
       apply (unfold is_graph_def)[1]
       apply (clarsimp simp: if_bool_eq_conj)+
-     apply (rule ccontr, erule notE)
+     apply (rule ccontr, erule_tac P="is_valid_ENInt_C s (d +\<^sub>p uint sc)" in notE)
      apply (unfold s_assms_inv_def is_graph_def is_dist_def)[1]
      apply (clarsimp simp: if_bool_eq_conj)+
      apply (rule arrlist_nth, (simp add: uint_nat unat_mono )+)
      apply (metis not_le word_less_nat_alt)
-    apply (rule impI, rule ccontr, erule notE)
+    apply (rule impI, rule ccontr, erule_tac P="is_valid_w32 s (PTR_COERCE(32 signed word \<rightarrow> 32 word) 
+           (p +\<^sub>p uint sc))" in notE)
     apply (unfold s_assms_inv_def is_graph_def is_pedge_def)[1]
     apply (clarsimp simp: if_bool_eq_conj)+
     apply (rule arrlist_nth, (simp add: uint_nat unat_mono )+)
@@ -2130,7 +2106,7 @@ lemma s_assms_spc':
        apply (subst is_inf_d_heap, simp, force, simp add: uint_nat)
       apply (rule conjI)
        apply (subgoal_tac "iP sc = heap_w32 s (PTR_COERCE(32 signed word \<rightarrow> 32 word) (p +\<^sub>p int (unat sc)))")
-        apply (simp add: range_2)
+        apply (simp add: sint_ucast)
        apply (subgoal_tac "int (unat sc) = uint sc")
         apply (force intro: pedge_abs_C_equiv_2)
        apply (simp add:uint_nat)
@@ -2155,6 +2131,84 @@ lemma s_assms_spc':
   apply (rule arrlist_nth, (simp add: uint_nat unat_mono )+)
   apply (metis not_le word_of_nat_le word_unat.Rep_inverse)
   done
+
+lemma s_assms_eq_math:
+  "s_assms_inv G sc d p n  \<longleftrightarrow> 
+   (sc \<in> verts (abs_IGraph G) \<and>
+    abs_IDist d sc \<noteq> \<infinity> \<and>
+    abs_IPedge p sc = None \<and>
+    abs_INum n sc = 0)"
+  apply safe
+      apply (unfold s_assms_inv_def abs_IGraph_def, clarsimp)[1]
+     apply (unfold s_assms_inv_def abs_IDist_def, clarsimp)[1]
+    apply (unfold s_assms_inv_def abs_IPedge_def, clarsimp)[1]
+  using word_msb_sint apply blast
+   apply (unfold s_assms_inv_def abs_INum_def, clarsimp, simp add: zero_enat_def)[1]
+  apply (unfold s_assms_inv_def abs_IGraph_def abs_IDist_def abs_INum_def abs_IPedge_def, clarsimp)
+   apply (simp add: unat_eq_zero word_msb_sint zero_enat_def)+
+  done
+
+definition parent_num_assms_inv :: 
+  "IGraph \<Rightarrow> IVertex \<Rightarrow> IENInt \<Rightarrow> IPEdge \<Rightarrow> IEInt  \<Rightarrow> 32 word \<Rightarrow> bool" where
+  "parent_num_assms_inv G s d p n k \<equiv>
+    \<forall>v < k. v \<noteq> s \<and> is_inf_d d v = 0 \<longrightarrow> 
+      sint (p v) \<ge> 0 \<and>
+      (\<exists> e. e = p v \<and> e < iedge_cnt G \<and>
+        v = snd (iedges G e) \<and>
+        is_inf_d d (fst (iedges G e)) \<le> 0 \<and>
+        is_inf_n n v = 0 \<and>
+        is_inf_n n (fst (iedges G e)) = 0 \<and>
+        cast_long (val_n n v) = cast_long (val_n n (fst (iedges G e))) + 1)"
+
+lemma parent_num_assms_step:
+  assumes v_less_max: "v < (max_word::32 word)"
+  shows "parent_num_assms_inv G s d p n (v + 1) \<longleftrightarrow> parent_num_assms_inv G s d p n v
+    \<and> (v \<noteq> s \<and> is_inf_d d v = 0 \<longrightarrow> 
+      sint (p v) \<ge> 0 \<and>
+      (\<exists> e. e = p v \<and> e < iedge_cnt G \<and>
+        v = snd (iedges G e) \<and>
+        is_inf_d d (fst (iedges G e)) \<le> 0 \<and>
+        is_inf_n n v = 0 \<and>
+        is_inf_n n (fst (iedges G e)) = 0 \<and>
+        cast_long (val_n n v) = cast_long (val_n n (fst (iedges G e))) + 1))"
+  unfolding parent_num_assms_inv_def apply safe
+  by (metis less_x_plus_1 max_word_max not_le v_less_max)+
+                  
+lemma parent_num_assms_le:
+  assumes leq: "j \<le> i" 
+  assumes parent_num_assms_i: "parent_num_assms_inv G s d p n i"
+  shows "parent_num_assms_inv G s d p n j"
+  using assms 
+  by (induct j) (auto simp add: parent_num_assms_inv_def)
+
+lemma parent_num_assms_spc':
+  "\<lbrace> P and 
+     (\<lambda>s. wf_digraph (abs_IGraph iG) \<and>
+          is_graph s iG g \<and>
+          is_dist s iG iD d \<and>
+          is_numm s iG iN n \<and>
+          is_pedge s iG iP p)\<rbrace>
+   parent_num_assms' g sc d p n
+   \<lbrace> (\<lambda>_ s. P s) And 
+     (\<lambda>rr s. rr \<noteq> 0 \<longleftrightarrow> parent_num_assms_inv iG sc iD iP iN (ivertex_cnt iG)) \<rbrace>!"
+  apply (clarsimp simp: parent_num_assms'_def)
+  apply (subst whileLoopE_add_inv [where 
+        M="\<lambda>(vv, s). unat (ivertex_cnt iG - vv)" and
+        I="\<lambda>vv s. P s \<and> parent_num_assms_inv iG sc iD iP iN vv \<and>
+                   vv \<le> ivertex_cnt iG \<and>
+                   wf_digraph (abs_IGraph iG) \<and>
+                   is_graph s iG g \<and>
+                   is_dist s iG iD d \<and>
+                   is_numm s iG iN n \<and>
+                   is_pedge s iG iP p"])
+  apply (simp add: skipE_def)
+  apply wp
+     apply (subst if_bool_eq_conj)+
+     apply simp
+     apply (rule conjI, rule impI, rule conjI, rule impI, rule conjI, rule impI, rule conjI)
+         apply blast
+
+
 
 end
 
